concurrency/hack-hash-table/Impl.i.dfy
@@ -1,4 +1,5 @@
 include "../framework/Mutex.s.dfy"
+include "CapacityAllocator.i.dfy"
 include "HTResource.i.dfy"
 include "Main.s.dfy"
 
@@ -8,33 +9,31 @@ module Impl refines Main {
   import opened HTResource
   import opened KeyValueType
   import opened Mutexes
+  import opened CapacityAllocatorTypes
+  import CAP = CapacityAllocator
 
   linear datatype Row = Row(
     entry: HTResource.Entry,
     linear resource: HTResource.R)
 
-  type HTMutex = Mutex<Row>
-  type MutexTable = seq<HTMutex>
+  type RowMutex = Mutex<Row>
+  type RowMutexTable = seq<RowMutex>
+
+  datatype Variables = Variables(rowMutexes: RowMutexTable, allocator: CAP.AllocatorMutexTable)
 
   function RowInv(index: nat, row: Row): bool
   {
     && Valid(row.resource)
     && 0 <= index as nat < FixedSize()
-    && row.resource == oneRowResource(index as nat, Info(row.entry, Free))
+    && row.resource == oneRowResource(index as nat, Info(row.entry, Free), 0)
   }
 
-  predicate Inv(o: MutexTable) {
-    && |o| == HTResource.FixedSize()
+  predicate Inv(v: Variables) {
+    && CAP.Inv(v.allocator)
+    && |v.rowMutexes| == HTResource.FixedSize()
     && (forall i | 0 <= i < FixedSize()
-      :: o[i].inv == ((row) => RowInv(i, row)))
+      :: v.rowMutexes[i].inv == ((row) => RowInv(i, row)))
   }
-
-  // predicate Init(s: ARS.R) {
-  //   && s.R?
-  //   && (forall i | 0 < i < |s.table| :: s.table[i] == Some(Info(Empty, Free)))
-  //   && s.tickets == multiset{}
-  //   && s.stubs == multiset{}
-  // }
 
   datatype Splitted = Splitted(r':ARS.R, ri:ARS.R)
 
@@ -49,32 +48,36 @@ module Impl refines Main {
   }
 
   method init(linear in_r: ARS.R)
-  returns (o: MutexTable, linear out_r: ARS.R)
+  returns (v: Variables, linear out_r: ARS.R)
   // requires ARS.Init(i)
-  ensures Inv(o)
+  ensures Inv(v)
   ensures out_r == unit()
   {
     linear var remaining_r := in_r;
-    o := [];
+    var rowMutexes : RowMutexTable:= [];
     var i:uint32 := 0;
     while i < FixedSizeImpl()
-      invariant i as int == |o| <= FixedSize()
-      invariant forall j:nat | j<i as int :: && o[j].inv == (row) => RowInv(j, row)
+      invariant i as int == |rowMutexes| <= FixedSize()
+      invariant forall j:nat | j<i as int :: && rowMutexes[j].inv == (row) => RowInv(j, row)
       invariant remaining_r.R?
       invariant remaining_r.tickets == multiset{}
       invariant remaining_r.stubs == multiset{} 
       invariant forall k:nat | k < i as int :: remaining_r.table[k].None?
       invariant forall l:nat | i as int <= l < |remaining_r.table| :: remaining_r.table[l] == Some(Info(Empty, Free))
+      invariant remaining_r.insert_capacity == Capacity()
     {
       ghost var splitted := Split(remaining_r, i as int);
       linear var ri;
       remaining_r, ri := ARS.split(remaining_r, splitted.r', splitted.ri);
       var m := new_mutex<Row>(Row(Empty, ri), (row) => RowInv(i as nat, row));
-      o := o + [m];
+      rowMutexes := rowMutexes + [m];
       i := i + 1;
     }
 
-    out_r := remaining_r;
+    var allocator: CAP.AllocatorMutexTable;
+    allocator, out_r := CAP.init(remaining_r);
+
+    v := Variables(rowMutexes, allocator);
 
     assert forall i:nat | i < FixedSize() :: out_r.table[i].None?;
     assert out_r == unit();
@@ -103,33 +106,37 @@ module Impl refines Main {
       else (dst as int - src as int)
   }
 
-  method doQuery(mt: MutexTable, input: Ifc.Input, rid: int,  /*ghost*/ linear in_r: ARS.R)
+  method doQuery(v: Variables, input: Ifc.Input, rid: int,  /*ghost*/ linear in_r: ARS.R)
   returns (output: Ifc.Output, linear out_r: ARS.R)
-    requires Inv(mt)
+    decreases *
+    requires Inv(v)
     requires input.QueryInput?
     requires isInputResource(in_r, rid, input)
     ensures out_r == ARS.output_stub(rid, output)
   {
+    var rm := v.rowMutexes;
     var query_ticket := Ticket(rid, input);
     var key := input.key;
     var hash_idx := hash(key);
     var slot_idx := hash_idx;
 
     linear var row; glinear var handle;
-    row, handle := mt[slot_idx].acquire();
+    row, handle := rm[slot_idx].acquire();
     linear var Row(entry, row_r) := row;
     linear var r := ARS.join(in_r, row_r);
 
-    ghost var r' := oneRowResource(hash_idx as nat, Info(entry, Querying(rid, key)));
+    ghost var r' := oneRowResource(hash_idx as nat, Info(entry, Querying(rid, key)), 0);
+    assert ProcessQueryTicket(r, r', query_ticket);
+
     var step := ProcessQueryTicketStep(query_ticket);
     r := easy_transform_step(r, r', step);
 
     while true 
-      invariant Inv(mt);
+      invariant Inv(v);
       invariant 0 <= slot_idx < FixedSizeImpl();
-      invariant r == oneRowResource(slot_idx as nat, Info(entry, Querying(rid, key)));
-      invariant handle.m == mt[slot_idx];
-      decreases DistanceToSlot(slot_idx, hash_idx);
+      invariant r == oneRowResource(slot_idx as nat, Info(entry, Querying(rid, key)), 0);
+      invariant handle.m == rm[slot_idx];
+      decreases *
     {
       var slot_idx' := getNextIndex(slot_idx);
 
@@ -156,27 +163,29 @@ module Impl refines Main {
       }
 
       if !step.QuerySkipStep? {
+        // this test is required for termination, but is not enforced by verification
+        // because we are using decreases *
         break;
       }
 
-      if slot_idx' == hash_idx {
-        QueryUnreachableState(r, slot_idx as nat);
-        break;
-      }
+      // if slot_idx' == hash_idx {
+      //   QueryUnreachableState(r, slot_idx as nat);
+      //   break;
+      // }
 
       linear var next_row; glinear var next_handle;
-      next_row, next_handle := mt[slot_idx'].acquire();
+      next_row, next_handle := rm[slot_idx'].acquire();
       linear var Row(next_entry, next_row_r) := next_row;
       r := ARS.join(r, next_row_r);
 
-      r' := twoRowsResource(slot_idx as nat, Info(entry, Free), slot_idx' as nat, Info(next_entry, Querying(rid, key)));
+      r' := twoRowsResource(slot_idx as nat, Info(entry, Free), slot_idx' as nat, Info(next_entry, Querying(rid, key)), 0);
       r := easy_transform_step(r, r', step);
 
       linear var rmutex;
-      ghost var left := oneRowResource(slot_idx' as nat, Info(next_entry, Querying(rid, key)));
-      ghost var right := oneRowResource(slot_idx as nat, Info(entry, Free));
+      ghost var left := oneRowResource(slot_idx' as nat, Info(next_entry, Querying(rid, key)), 0);
+      ghost var right := oneRowResource(slot_idx as nat, Info(entry, Free), 0);
       r, rmutex := ARS.split(r, left, right);
-      mt[slot_idx].release(Row(entry, rmutex), handle);
+      rm[slot_idx].release(Row(entry, rmutex), handle);
 
       slot_idx := slot_idx';
       entry := next_entry;
@@ -190,19 +199,56 @@ module Impl refines Main {
     linear var rmutex;
     r, rmutex := ARS.split(r, 
       ARS.output_stub(rid, output), 
-      oneRowResource(slot_idx as nat, Info(entry, Free)));
-    mt[slot_idx].release(Row(entry, rmutex), handle);
+      oneRowResource(slot_idx as nat, Info(entry, Free), 0));
+    rm[slot_idx].release(Row(entry, rmutex), handle);
 
     out_r := r;
   }
 
-  method doInsert(mt: MutexTable, input: Ifc.Input, rid: int, /*ghost*/ linear in_r: ARS.R)
+  method acquireCapacity(v: Variables, thread_id: uint32)
+  returns (linear cap: AllocatorBin, glinear cap_handle: MutexHandle<AllocatorBin>, tid: uint32)
+    decreases *
+    requires Inv(v)
+    ensures cap.resource == unit().(insert_capacity := cap.count as nat)
+    ensures 0 < cap.count
+    ensures tid < CAP.BinCountImpl()
+    ensures cap_handle.m == v.allocator[tid]
+  {
+    // thread_id is a hint for the bin we're supposed to use. 
+    // tid is the actual place we found the capacity (in case we had to steal it from someone else) 
+    tid := if thread_id >= CAP.BinCountImpl() then 0 else thread_id;
+    cap, cap_handle := v.allocator[tid].acquire();
+
+    while true
+      invariant tid < CAP.BinCountImpl()
+      invariant cap.resource == unit().(insert_capacity := cap.count as nat)
+      invariant cap_handle.m == v.allocator[tid]
+      decreases *
+    {
+      if 0 < cap.count {
+        break;
+      }
+
+      v.allocator[tid].release(cap, cap_handle);
+
+      tid := tid + 1;
+      tid := if tid >= CAP.BinCountImpl() then 0 else tid;
+
+      cap, cap_handle := v.allocator[tid].acquire();
+    }
+  }
+
+  method doInsert(v: Variables, input: Ifc.Input, rid: int, /*ghost*/ linear in_r: ARS.R, thread_id: uint32)
   returns (output: Ifc.Output, linear out_r: ARS.R)
-    requires Inv(mt)
+    requires Inv(v)
     requires input.InsertInput?
     requires isInputResource(in_r, rid, input)
     ensures out_r == ARS.output_stub(rid, output)
+    decreases *
   {
+    var rm := v.rowMutexes;
+    var allocator := v.allocator;
+
     var query_ticket := Ticket(rid, input);
     var key, inital_key := input.key, input.key;
     var kv := KV(key, input.value);
@@ -212,24 +258,32 @@ module Impl refines Main {
     var initial_hash_idx := hash_idx;
     var slot_idx := hash_idx;
 
+    linear var cap; glinear var cap_handle; var tid;
+    cap, cap_handle, tid := acquireCapacity(v, thread_id);
+
+    linear var AllocatorBin(count, cap_r) := cap;
+    linear var r := ARS.join(in_r, cap_r);
+
     linear var row; glinear var handle;
-    row, handle := mt[slot_idx].acquire();
+    row, handle := rm[slot_idx].acquire();
     linear var Row(entry, row_r) := row;
-    linear var r := ARS.join(in_r, row_r);
+    r := ARS.join(r, row_r);
+
+    count := count - 1;
 
     var step := ProcessInsertTicketStep(query_ticket);
-    ghost var r' := oneRowResource(hash_idx as nat, Info(entry, Inserting(rid, kv, inital_key)));
+    ghost var r' := oneRowResource(hash_idx as nat, Info(entry, Inserting(rid, kv, inital_key)), count as nat);
     r := easy_transform_step(r, r', step);
     linear var rmutex;
 
     while true 
-      invariant Inv(mt);
+      invariant Inv(v);
       invariant 0 <= slot_idx < FixedSizeImpl()
-      invariant r == oneRowResource(slot_idx as nat, Info(entry, Inserting(rid, kv, inital_key)))
+      invariant r == oneRowResource(slot_idx as nat, Info(entry, Inserting(rid, kv, inital_key)), count as nat)
       invariant kv.key == key
       invariant hash_idx == hash(key)
-      invariant handle.m == mt[slot_idx];
-      decreases DistanceToSlot(slot_idx, initial_hash_idx)
+      invariant handle.m == rm[slot_idx];
+      decreases *
     {
       var slot_idx' := getNextIndex(slot_idx);
       var new_kv;
@@ -257,13 +311,8 @@ module Impl refines Main {
         break;
       }
 
-      if slot_idx' == initial_hash_idx {
-        InsertUnreachableState(r, slot_idx as nat);
-        break;
-      }
-
       linear var next_row; glinear var next_handle;
-      next_row, next_handle := mt[slot_idx'].acquire();
+      next_row, next_handle := rm[slot_idx'].acquire();
       linear var Row(next_entry, next_row_r) := next_row;
       r := ARS.join(r, next_row_r);
 
@@ -273,14 +322,14 @@ module Impl refines Main {
         key := new_kv.key;
       }
   
-      r' := twoRowsResource(slot_idx as nat, Info(entry, Free), slot_idx' as nat, Info(next_entry, Inserting(rid, kv, inital_key)));
+      r' := twoRowsResource(slot_idx as nat, Info(entry, Free), slot_idx' as nat, Info(next_entry, Inserting(rid, kv, inital_key)), count as nat);
       r := easy_transform_step(r, r', step);
 
-      ghost var left := oneRowResource(slot_idx' as nat, Info(next_entry, Inserting(rid, kv, inital_key)));
-      ghost var right := oneRowResource(slot_idx as nat, Info(entry, Free));
+      ghost var left := oneRowResource(slot_idx' as nat, Info(next_entry, Inserting(rid, kv, inital_key)), count as nat);
+      ghost var right := oneRowResource(slot_idx as nat, Info(entry, Free), 0);
 
       r, rmutex := ARS.split(r, left, right);
-      mt[slot_idx].release(Row(entry, rmutex), handle);
+      rm[slot_idx].release(Row(entry, rmutex), handle);
 
       slot_idx := slot_idx';
       entry := next_entry;
@@ -289,242 +338,251 @@ module Impl refines Main {
     }
 
     // assert step.InsertDoneStep? || step.InsertUpdateStep?;
-    r' := R(oneRowTable(slot_idx as nat, Info(Full(kv), Free)), 0, multiset{}, multiset{Stub(rid, output)});
+    count := if step.InsertDoneStep? then count else count + 1;
+    r' := R(oneRowTable(slot_idx as nat, Info(Full(kv), Free)), count as nat, multiset{}, multiset{Stub(rid, output)});
     r := easy_transform_step(r, r', step);
-
-    r, rmutex := ARS.split(r, ARS.output_stub(rid, output), 
-      oneRowResource(slot_idx as nat, Info(Full(kv), Free)));
-    mt[slot_idx].release(Row(Full(kv), rmutex), handle);
-
-    out_r := r;
-  }
-
-  method doRemoveFound(mt: MutexTable, rid: int, 
-    slot_idx: uint32,
-    hash_idx: uint32,
-    inital_key: Key,
-    entry: Entry,
-    glinear handle: MutexHandle<Row>,
-    /*ghost*/ linear r: ARS.R)
-  returns (output: Ifc.Output, linear out_r: ARS.R)
-    requires Inv(mt)
-    requires 0 <= slot_idx < FixedSizeImpl()
-    requires 0 <= hash_idx < FixedSizeImpl()
-    requires r == oneRowResource(slot_idx as nat, Info(entry, Removing(rid, inital_key)));
-    requires entry.Full? && entry.kv.key == inital_key
-    requires hash(inital_key) == hash_idx
-    requires handle.m == mt[slot_idx]
-    ensures out_r == ARS.output_stub(rid, output)
-  {
-    var slot_idx := slot_idx;
-    var slot_idx' := getNextIndex(slot_idx);
-
-    glinear var handle := handle;
-    linear var rmutex;
-
-    linear var next_row; glinear var next_handle;
-    next_row, next_handle := mt[slot_idx'].acquire();
-    linear var Row(next_entry, next_row_r) := next_row;
-    linear var r := ARS.join(r, next_row_r);
-
-    var step := RemoveFoundItStep(slot_idx as nat);
-    var r' := twoRowsResource(slot_idx as nat, Info(Empty, RemoveTidying(rid, inital_key)), slot_idx' as nat, Info(next_entry, Free));
-    r := easy_transform_step(r, r', step);
-
-    while true
-      invariant Inv(mt);
-      invariant 0 <= slot_idx < FixedSizeImpl()
-      invariant r == twoRowsResource(slot_idx as nat, Info(Empty, RemoveTidying(rid, inital_key)), NextPos(slot_idx as nat), Info(next_entry, Free))
-      invariant handle.m == mt[slot_idx]
-      invariant next_handle.m == mt[NextPos(slot_idx as nat)]
-      decreases DistanceToSlot(slot_idx, hash_idx)
-    {
-      slot_idx' := getNextIndex(slot_idx);
-
-      if next_entry.Empty? || (next_entry.Full? && hash(next_entry.kv.key) == slot_idx') {
-        assert DoneTidying(r, slot_idx as nat);
-        break;
-      }
-  
-      if slot_idx' == hash_idx {
-        RemoveTidyUnreachableState(r, slot_idx as nat);
-        break;
-      }
-
-      ghost var r' := twoRowsResource(
-        slot_idx as nat, Info(next_entry, Free),
-        slot_idx' as nat, Info(Empty, RemoveTidying(rid, inital_key)));
-      r := easy_transform_step(r, r', RemoveTidyStep(slot_idx as nat));
-
-      ghost var left := oneRowResource(slot_idx' as nat, Info(Empty, RemoveTidying(rid, inital_key)));
-      ghost var right := oneRowResource(slot_idx as nat, Info(next_entry, Free));
-
-      r, rmutex := ARS.split(r, left, right);
-      mt[slot_idx].release(Row(next_entry, rmutex), handle);
-
-      slot_idx := slot_idx';
-      slot_idx' := getNextIndex(slot_idx);
-      handle := next_handle;
-
-      next_row, next_handle := mt[slot_idx'].acquire();
-      linear var Row(next_entry', next_row_r) := next_row;
-      next_entry := next_entry';
-      r := ARS.join(r, next_row_r);
-    }
-
-    assert DoneTidying(r, slot_idx as nat);
-
-    slot_idx' := getNextIndex(slot_idx);
-    output := MapIfc.RemoveOutput(true);
-    r' := R(
-      twoRowsTable(slot_idx as nat, Info(Empty, Free), slot_idx' as nat, Info(next_entry, Free)),
-      0,
-      multiset{},
-      multiset{ Stub(rid, output) }
-    );
-
-    step := RemoveDoneStep(slot_idx as nat);
-    r := easy_transform_step(r, r', step);
-
-    ghost var left := R(
-      oneRowTable(slot_idx' as nat, Info(next_entry, Free)),
-      0,
-      multiset{},
-      multiset{ Stub(rid, output) });
-    ghost var right := oneRowResource(slot_idx as nat, Info(Empty, Free));
-
-    r, rmutex := ARS.split(r, left, right);
-    mt[slot_idx].release(Row(Empty, rmutex), handle);
 
     r, rmutex := ARS.split(r, 
+      ARS.output_stub(rid, output).(insert_capacity := count as nat), 
+      oneRowResource(slot_idx as nat, Info(Full(kv), Free), 0));
+    rm[slot_idx].release(Row(Full(kv), rmutex), handle);
+
+    linear var rcap;
+    r, rcap := ARS.split(r,
       ARS.output_stub(rid, output), 
-      oneRowResource(slot_idx' as nat, Info(next_entry, Free)));
-    mt[slot_idx'].release(Row(next_entry, rmutex), next_handle);
+      unit().(insert_capacity := count as nat));
+
+    allocator[tid].release(AllocatorBin(count, rcap), cap_handle);
 
     out_r := r;
   }
 
-  method doRemove(mt: MutexTable, input: Ifc.Input, rid: int, /*ghost*/ linear in_r: ARS.R)
-    returns (output: Ifc.Output, linear out_r: ARS.R)
-    requires Inv(mt)
-    requires input.RemoveInput?
-    requires isInputResource(in_r, rid, input)
-    ensures out_r == ARS.output_stub(rid, output)
-  {
-    var query_ticket := Ticket(rid, input);
-    var key := input.key;
+  // method doRemoveFound(v: Variables, rid: int, 
+  //   slot_idx: uint32,
+  //   hash_idx: uint32,
+  //   inital_key: Key,
+  //   entry: Entry,
+  //   glinear handle: MutexHandle<Row>,
+  //   /*ghost*/ linear r: ARS.R)
+  // returns (output: Ifc.Output, linear out_r: ARS.R)
+  //   requires Inv(mt)
+  //   requires 0 <= slot_idx < FixedSizeImpl()
+  //   requires 0 <= hash_idx < FixedSizeImpl()
+  //   requires r == oneRowResource(slot_idx as nat, Info(entry, Removing(rid, inital_key)));
+  //   requires entry.Full? && entry.kv.key == inital_key
+  //   requires hash(inital_key) == hash_idx
+  //   requires handle.m == mt[slot_idx]
+  //   ensures out_r == ARS.output_stub(rid, output)
+  // {
+  //   var slot_idx := slot_idx;
+  //   var slot_idx' := getNextIndex(slot_idx);
 
-    var hash_idx := hash(key); var slot_idx := hash_idx;
+  //   glinear var handle := handle;
+  //   linear var rmutex;
 
-    linear var row; glinear var handle;
-    row, handle := mt[slot_idx].acquire();
+  //   linear var next_row; glinear var next_handle;
+  //   next_row, next_handle := mt[slot_idx'].acquire();
+  //   linear var Row(next_entry, next_row_r) := next_row;
+  //   linear var r := ARS.join(r, next_row_r);
 
-    linear var Row(entry, row_r) := row;
-    linear var r := ARS.join(in_r, row_r);
+  //   var step := RemoveFoundItStep(slot_idx as nat);
+  //   var r' := twoRowsResource(slot_idx as nat, Info(Empty, RemoveTidying(rid, inital_key)), slot_idx' as nat, Info(next_entry, Free));
+  //   r := easy_transform_step(r, r', step);
 
-    var slot_idx' :uint32;
-    linear var rmutex;
+  //   while true
+  //     invariant Inv(mt);
+  //     invariant 0 <= slot_idx < FixedSizeImpl()
+  //     invariant r == twoRowsResource(slot_idx as nat, Info(Empty, RemoveTidying(rid, inital_key)), NextPos(slot_idx as nat), Info(next_entry, Free))
+  //     invariant handle.m == mt[slot_idx]
+  //     invariant next_handle.m == mt[NextPos(slot_idx as nat)]
+  //     decreases DistanceToSlot(slot_idx, hash_idx)
+  //   {
+  //     slot_idx' := getNextIndex(slot_idx);
 
-    ghost var r' := oneRowResource(hash_idx as nat, Info(entry, Removing(rid, key)));
-    var step : Step := ProcessRemoveTicketStep(query_ticket);
-    r := easy_transform_step(r, r', step);
+  //     if next_entry.Empty? || (next_entry.Full? && hash(next_entry.kv.key) == slot_idx') {
+  //       assert DoneTidying(r, slot_idx as nat);
+  //       break;
+  //     }
+  
+  //     if slot_idx' == hash_idx {
+  //       RemoveTidyUnreachableState(r, slot_idx as nat);
+  //       break;
+  //     }
 
-    while true 
-      invariant Inv(mt);
-      invariant 0 <= slot_idx < FixedSizeImpl();
-      invariant r == oneRowResource(slot_idx as nat, Info(entry, Removing(rid, key)))
-      invariant step.RemoveNotFoundStep? ==> 
-        (entry.Full? && shouldHashGoBefore(hash_idx, hash(entry.kv.key), slot_idx))
-      invariant step.RemoveTidyStep? ==> (
-        && TidyEnabled(r, slot_idx as nat)
-        && KnowRowIsFree(r, NextPos(slot_idx as nat)))
-      invariant handle.m == mt[slot_idx]
-      decreases DistanceToSlot(slot_idx, hash_idx)
-    {
-      var slot_idx' := getNextIndex(slot_idx);
+  //     ghost var r' := twoRowsResource(
+  //       slot_idx as nat, Info(next_entry, Free),
+  //       slot_idx' as nat, Info(Empty, RemoveTidying(rid, inital_key)));
+  //     r := easy_transform_step(r, r', RemoveTidyStep(slot_idx as nat));
 
-      match entry {
-        case Empty => {
-          step := RemoveNotFoundStep(slot_idx as nat);
-        }
-        case Full(KV(entry_key, value)) => {
-          if entry_key == key {
-            step := RemoveFoundItStep(slot_idx as nat);
-          } else {
-            var should_go_before := shouldHashGoBefore(hash_idx, hash(entry_key), slot_idx);
+  //     ghost var left := oneRowResource(slot_idx' as nat, Info(Empty, RemoveTidying(rid, inital_key)));
+  //     ghost var right := oneRowResource(slot_idx as nat, Info(next_entry, Free));
 
-            if !should_go_before {
-              step := RemoveSkipStep(slot_idx as nat);
-            } else {
-              step := RemoveNotFoundStep(slot_idx as nat);
-            }
-          }
-        }
-      }
+  //     r, rmutex := ARS.split(r, left, right);
+  //     mt[slot_idx].release(Row(next_entry, rmutex), handle);
 
-      if slot_idx' == hash_idx {
-        RemoveUnreachableState(r, slot_idx as nat);
-        break;
-      }
+  //     slot_idx := slot_idx';
+  //     slot_idx' := getNextIndex(slot_idx);
+  //     handle := next_handle;
 
-      if step.RemoveNotFoundStep? || step.RemoveFoundItStep? {
-        break;
-      }
+  //     next_row, next_handle := mt[slot_idx'].acquire();
+  //     linear var Row(next_entry', next_row_r) := next_row;
+  //     next_entry := next_entry';
+  //     r := ARS.join(r, next_row_r);
+  //   }
 
-      linear var next_row; glinear var next_handle;
-      next_row, next_handle := mt[slot_idx'].acquire();
-      linear var Row(next_entry, next_row_r) := next_row;
-      r := ARS.join(r, next_row_r);
+  //   assert DoneTidying(r, slot_idx as nat);
 
-      r' := twoRowsResource(slot_idx as nat, Info(entry, Free), slot_idx' as nat, Info(next_entry, Removing(rid, key)));
-      r := easy_transform_step(r, r', step);
+  //   slot_idx' := getNextIndex(slot_idx);
+  //   output := MapIfc.RemoveOutput(true);
+  //   r' := R(
+  //     twoRowsTable(slot_idx as nat, Info(Empty, Free), slot_idx' as nat, Info(next_entry, Free)),
+  //     0,
+  //     multiset{},
+  //     multiset{ Stub(rid, output) }
+  //   );
 
-      ghost var left := oneRowResource(slot_idx' as nat, Info(next_entry, Removing(rid, key)));
-      ghost var right := oneRowResource(slot_idx as nat, Info(entry, Free));
-      r, rmutex := ARS.split(r, left, right);
-      mt[slot_idx].release(Row(entry, rmutex), handle);
+  //   step := RemoveDoneStep(slot_idx as nat);
+  //   r := easy_transform_step(r, r', step);
 
-      slot_idx := slot_idx';
-      entry := next_entry;
-      handle := next_handle;
-    }
+  //   ghost var left := R(
+  //     oneRowTable(slot_idx' as nat, Info(next_entry, Free)),
+  //     0,
+  //     multiset{},
+  //     multiset{ Stub(rid, output) });
+  //   ghost var right := oneRowResource(slot_idx as nat, Info(Empty, Free));
 
-    if step.RemoveNotFoundStep? {
-      output := MapIfc.RemoveOutput(false);
-      r' := R(oneRowTable(slot_idx as nat, Info(entry, Free)), 0, multiset{}, multiset{Stub(rid, output)}); 
-      r := easy_transform_step(r, r', step);
-      ghost var left := ARS.output_stub(rid, output);
-      ghost var right := oneRowResource(slot_idx as nat, Info(entry, Free));
-      r, rmutex := ARS.split(r, left, right);
-      mt[slot_idx].release(Row(entry, rmutex), handle);
-    } else {
-      output, r := doRemoveFound(mt, rid, slot_idx, hash_idx, key, entry, handle, r);
-    }
+  //   r, rmutex := ARS.split(r, left, right);
+  //   mt[slot_idx].release(Row(Empty, rmutex), handle);
 
-    out_r := r;
-  }
+  //   r, rmutex := ARS.split(r, 
+  //     ARS.output_stub(rid, output), 
+  //     oneRowResource(slot_idx' as nat, Info(next_entry, Free)));
+  //   mt[slot_idx'].release(Row(next_entry, rmutex), next_handle);
 
-  method call(o: MutexTable, input: Ifc.Input,
-      rid: int, linear in_r: ARS.R, thread_id: nat)
-    returns (output: Ifc.Output, linear out_r: ARS.R)
-  // requires Inv(o)
-  // requires ticket == ARS.input_ticket(rid, key)
-    ensures out_r == ARS.output_stub(rid, output)
-  {
-    // Find the ticket.
-    assert |in_r.tickets| == 1;
-    var the_ticket :| the_ticket in in_r.tickets;
+  //   out_r := r;
+  // }
 
-    if the_ticket.input.QueryInput? {
-      output, out_r := doQuery(o, input, rid, in_r);
-    } else if the_ticket.input.InsertInput? {
-      output, out_r := doInsert(o, input, rid, in_r);
-    } else if the_ticket.input.RemoveInput? {
-      output, out_r := doRemove(o, input, rid, in_r);
-    } else {
-      out_r := in_r;
-      assert false;
-    }
-  }
+  // method doRemove(v: Variables, input: Ifc.Input, rid: int, /*ghost*/ linear in_r: ARS.R)
+  //   returns (output: Ifc.Output, linear out_r: ARS.R)
+  //   requires Inv(mt)
+  //   requires input.RemoveInput?
+  //   requires isInputResource(in_r, rid, input)
+  //   ensures out_r == ARS.output_stub(rid, output)
+  // {
+  //   var query_ticket := Ticket(rid, input);
+  //   var key := input.key;
+
+  //   var hash_idx := hash(key); var slot_idx := hash_idx;
+
+  //   linear var row; glinear var handle;
+  //   row, handle := mt[slot_idx].acquire();
+
+  //   linear var Row(entry, row_r) := row;
+  //   linear var r := ARS.join(in_r, row_r);
+
+  //   var slot_idx' :uint32;
+  //   linear var rmutex;
+
+  //   ghost var r' := oneRowResource(hash_idx as nat, Info(entry, Removing(rid, key)));
+  //   var step : Step := ProcessRemoveTicketStep(query_ticket);
+  //   r := easy_transform_step(r, r', step);
+
+  //   while true 
+  //     invariant Inv(mt);
+  //     invariant 0 <= slot_idx < FixedSizeImpl();
+  //     invariant r == oneRowResource(slot_idx as nat, Info(entry, Removing(rid, key)))
+  //     invariant step.RemoveNotFoundStep? ==> 
+  //       (entry.Full? && shouldHashGoBefore(hash_idx, hash(entry.kv.key), slot_idx))
+  //     invariant step.RemoveTidyStep? ==> (
+  //       && TidyEnabled(r, slot_idx as nat)
+  //       && KnowRowIsFree(r, NextPos(slot_idx as nat)))
+  //     invariant handle.m == mt[slot_idx]
+  //     decreases DistanceToSlot(slot_idx, hash_idx)
+  //   {
+  //     var slot_idx' := getNextIndex(slot_idx);
+
+  //     match entry {
+  //       case Empty => {
+  //         step := RemoveNotFoundStep(slot_idx as nat);
+  //       }
+  //       case Full(KV(entry_key, value)) => {
+  //         if entry_key == key {
+  //           step := RemoveFoundItStep(slot_idx as nat);
+  //         } else {
+  //           var should_go_before := shouldHashGoBefore(hash_idx, hash(entry_key), slot_idx);
+
+  //           if !should_go_before {
+  //             step := RemoveSkipStep(slot_idx as nat);
+  //           } else {
+  //             step := RemoveNotFoundStep(slot_idx as nat);
+  //           }
+  //         }
+  //       }
+  //     }
+
+  //     if slot_idx' == hash_idx {
+  //       RemoveUnreachableState(r, slot_idx as nat);
+  //       break;
+  //     }
+
+  //     if step.RemoveNotFoundStep? || step.RemoveFoundItStep? {
+  //       break;
+  //     }
+
+  //     linear var next_row; glinear var next_handle;
+  //     next_row, next_handle := mt[slot_idx'].acquire();
+  //     linear var Row(next_entry, next_row_r) := next_row;
+  //     r := ARS.join(r, next_row_r);
+
+  //     r' := twoRowsResource(slot_idx as nat, Info(entry, Free), slot_idx' as nat, Info(next_entry, Removing(rid, key)));
+  //     r := easy_transform_step(r, r', step);
+
+  //     ghost var left := oneRowResource(slot_idx' as nat, Info(next_entry, Removing(rid, key)));
+  //     ghost var right := oneRowResource(slot_idx as nat, Info(entry, Free));
+  //     r, rmutex := ARS.split(r, left, right);
+  //     mt[slot_idx].release(Row(entry, rmutex), handle);
+
+  //     slot_idx := slot_idx';
+  //     entry := next_entry;
+  //     handle := next_handle;
+  //   }
+
+  //   if step.RemoveNotFoundStep? {
+  //     output := MapIfc.RemoveOutput(false);
+  //     r' := R(oneRowTable(slot_idx as nat, Info(entry, Free)), 0, multiset{}, multiset{Stub(rid, output)}); 
+  //     r := easy_transform_step(r, r', step);
+  //     ghost var left := ARS.output_stub(rid, output);
+  //     ghost var right := oneRowResource(slot_idx as nat, Info(entry, Free));
+  //     r, rmutex := ARS.split(r, left, right);
+  //     mt[slot_idx].release(Row(entry, rmutex), handle);
+  //   } else {
+  //     output, r := doRemoveFound(mt, rid, slot_idx, hash_idx, key, entry, handle, r);
+  //   }
+
+  //   out_r := r;
+  // }
+
+  // method call(o: MutexTable, input: Ifc.Input,
+  //     rid: int, linear in_r: ARS.R, thread_id: nat)
+  //   returns (output: Ifc.Output, linear out_r: ARS.R)
+  // // requires Inv(o)
+  // // requires ticket == ARS.input_ticket(rid, key)
+  //   ensures out_r == ARS.output_stub(rid, output)
+  // {
+  //   // Find the ticket.
+  //   assert |in_r.tickets| == 1;
+  //   var the_ticket :| the_ticket in in_r.tickets;
+
+  //   if the_ticket.input.QueryInput? {
+  //     output, out_r := doQuery(o, input, rid, in_r);
+  //   } else if the_ticket.input.InsertInput? {
+  //     output, out_r := doInsert(o, input, rid, in_r);
+  //   } else if the_ticket.input.RemoveInput? {
+  //     output, out_r := doRemove(o, input, rid, in_r);
+  //   } else {
+  //     out_r := in_r;
+  //     assert false;
+  //   }
+  // }
 }
 
