concurrency/hack-hash-table/Main.s.dfy
@@ -4,18 +4,18 @@ abstract module Main {
   import ARS = HTResource
   import Ifc = MapIfc
 
-  type MutexTable(==,!new) // using this name so the impl is more readable
-  predicate Inv(o: MutexTable)
+  type Variables(==,!new) // using this name so the impl is more readable
+  predicate Inv(v: Variables)
 
   method init(linear in_r: ARS.R)
-  returns (o: MutexTable, linear out_r: ARS.R)
+  returns (v: Variables, linear out_r: ARS.R)
   requires ARS.Init(in_r)
-  ensures Inv(o)
+  ensures Inv(v)
 
-  method call(o: MutexTable, input: Ifc.Input,
+  method call(v: Variables, input: Ifc.Input,
       rid: int, linear in_r: ARS.R, thread_id: nat)
   returns (output: Ifc.Output, linear out_r: ARS.R)
-  requires Inv(o)
+  requires Inv(v)
   requires in_r == ARS.input_ticket(rid, input)
   ensures out_r == ARS.output_stub(rid, output)
 }
